Reorganized files and build proper call stacks

05TreeCode/TreeCode.thy
@@ -2,64 +2,52 @@ theory TreeCode
   imports "../00Utils/Environment"
 begin
 
-datatype tree_return =
-    TReturn
-  | TJump
-
 datatype tree_code = 
   TLookup nat
   | TPushCon nat
-  | TPushLam "tree_code list" tree_return
+  | TPushLam "tree_code list"
   | TApply
 
 datatype tclosure = 
   TConst nat
-  | TLam "tclosure list" "tree_code list" tree_return
+  | TLam "tclosure list" "tree_code list"
 
-type_synonym tree_stack_frame = "tclosure list \<times> tree_code list \<times> tree_return"
+type_synonym tree_stack_frame = "tclosure list \<times> tree_code list"
 
 datatype tree_code_state = TS "tclosure list" "tree_stack_frame list"
 
 inductive evalt :: "tree_code_state \<Rightarrow> tree_code_state \<Rightarrow> bool" (infix "\<leadsto>\<^sub>t" 50) where
   evt_lookup [simp]: "lookup env x = Some v \<Longrightarrow> 
-    TS vs ((env, TLookup x # cd, r) # sfs) \<leadsto>\<^sub>t TS (v # vs) ((env, cd, r) # sfs)"
-| evt_pushcon [simp]: "TS vs ((env, TPushCon k # cd, r) # sfs) \<leadsto>\<^sub>t 
-    TS (TConst k # vs) ((env, cd, r) # sfs)"
-| evt_pushlam [simp]: "TS vs ((env, TPushLam cd' r' # cd, r) # sfs) \<leadsto>\<^sub>t 
-    TS (TLam env cd' r' # vs) ((env, cd, r) # sfs)"
-| evt_apply [simp]: "TS (v # TLam env cd' r' # vs) ((env, TApply # cd, r) # sfs) \<leadsto>\<^sub>t 
-    TS vs ((v # env, cd', r') # (env, cd, r) # sfs)"
-| evt_return [simp]: "TS vs ((env, [], TReturn) # sfs) \<leadsto>\<^sub>t TS vs sfs"
-| evt_jump [simp]: "TS (v # TLam env' cd' r' # vs) ((env, [], TJump) # sfs) \<leadsto>\<^sub>t 
-    TS vs ((v # env', cd', r') # sfs)"
+    TS vs ((env, TLookup x # cd) # sfs) \<leadsto>\<^sub>t TS (v # vs) ((env, cd) # sfs)"
+| evt_pushcon [simp]: "TS vs ((env, TPushCon k # cd) # sfs) \<leadsto>\<^sub>t TS (TConst k # vs) ((env, cd) # sfs)"
+| evt_pushlam [simp]: "TS vs ((env, TPushLam cd' # cd) # sfs) \<leadsto>\<^sub>t 
+    TS (TLam env cd' # vs) ((env, cd) # sfs)"
+| evt_apply [simp]: "TS (v # TLam env cd' # vs) ((env, TApply # cd) # sfs) \<leadsto>\<^sub>t 
+    TS vs ((v # env, cd') # (env, cd) # sfs)"
+| evt_return [simp]: "TS vs ((env, []) # sfs) \<leadsto>\<^sub>t TS vs sfs"
 
 theorem determinismt: "\<Sigma> \<leadsto>\<^sub>t \<Sigma>' \<Longrightarrow> \<Sigma> \<leadsto>\<^sub>t \<Sigma>'' \<Longrightarrow> \<Sigma>' = \<Sigma>''"
 proof (induction \<Sigma> \<Sigma>' rule: evalt.induct)
-  case (evt_lookup env x v vs cd r sfs)
+  case (evt_lookup env x v vs cd sfs)
   from evt_lookup(2, 1) show ?case 
-    by (induction "TS vs ((env, TLookup x # cd, r) # sfs)" \<Sigma>'' rule: evalt.induct) simp_all 
+    by (induction "TS vs ((env, TLookup x # cd) # sfs)" \<Sigma>'' rule: evalt.induct) simp_all 
 next
-  case (evt_pushcon vs env k cd r sfs)
+  case (evt_pushcon vs env k cd sfs)
   thus ?case 
-    by (induction "TS vs ((env, TPushCon k # cd, r) # sfs)" \<Sigma>'' rule: evalt.induct) simp_all 
+    by (induction "TS vs ((env, TPushCon k # cd) # sfs)" \<Sigma>'' rule: evalt.induct) simp_all 
 next
-  case (evt_pushlam vs env cd' r' cd r sfs)
+  case (evt_pushlam vs env cd' cd sfs)
   thus ?case 
-    by (induction "TS vs ((env, TPushLam cd' r' # cd, r) # sfs)" \<Sigma>'' rule: evalt.induct) simp_all 
+    by (induction "TS vs ((env, TPushLam cd' # cd) # sfs)" \<Sigma>'' rule: evalt.induct) simp_all 
 next
-  case (evt_apply v env cd' r' vs cd r sfs)
+  case (evt_apply v env cd' vs cd sfs)
   thus ?case 
-    by (induction "TS (v # TLam env cd' r' # vs) ((env, TApply # cd, r) # sfs)" \<Sigma>'' 
+    by (induction "TS (v # TLam env cd' # vs) ((env, TApply # cd) # sfs)" \<Sigma>'' 
         rule: evalt.induct) 
        simp_all 
 next
   case (evt_return vs env sfs)
-  thus ?case by (induction "TS vs ((env, [], TReturn) # sfs)" \<Sigma>'' rule: evalt.induct) simp_all 
-next
-  case (evt_jump v env' cd' r' vs env sfs)
-  thus ?case 
-    by (induction "TS (v # TLam env' cd' r' # vs) ((env, [], TJump) # sfs)" \<Sigma>'' rule: evalt.induct) 
-       simp_all 
+  thus ?case by (induction "TS vs ((env, []) # sfs)" \<Sigma>'' rule: evalt.induct) simp_all 
 qed
 
 end
