08HeapMemory/HeapConversion.thy
@@ -15,17 +15,21 @@ fun unheap_closure :: "hclosure heap \<Rightarrow> ptr \<Rightarrow> bclosure" w
     | HLam env pc \<Rightarrow> 
         BLam (if stack_below x env then map (unheap_closure h) env else undefined) pc)"
 
+fun unheap_stack :: "hclosure heap \<Rightarrow> (ptr list \<times> nat) list \<Rightarrow> (bclosure list \<times> nat) list" where
+  "unheap_stack h [] = []"
+| "unheap_stack h ((env, pc) # sfs) = ((map (unheap_closure h) env, pc) # unheap_stack h sfs)"
+
 primrec unheap :: "heap_state \<Rightarrow> byte_code_state" where
-  "unheap (HS h vs envs pcs cd) = 
-    BS (map (unheap_closure h) vs) (map (map (unheap_closure h)) envs) pcs cd"
+  "unheap (HS h vs sfs cd) = 
+    BS (map (unheap_closure h) vs) (unheap_stack h sfs) cd"
 
 primrec bounded_closure :: "hclosure heap \<Rightarrow> ptr \<Rightarrow> hclosure \<Rightarrow> bool" where
   "bounded_closure h x (HConst k) = True"
 | "bounded_closure h x (HLam env pc) = (stack_contains h env \<and> stack_below x env)"
 
 primrec heap_structured :: "heap_state \<Rightarrow> bool" where
-  "heap_structured (HS h vs envs pcs cd) = (heap_all (bounded_closure h) h \<and>
-    stack_contains h vs \<and> env_contains h envs)"
+  "heap_structured (HS h vs sfs cd) = (heap_all (bounded_closure h) h \<and>
+    stack_contains h vs \<and> env_contains h (map fst sfs))"
 
 lemma [simp]: "halloc h a = (h', x) \<Longrightarrow> bounded_closure h y c \<Longrightarrow> bounded_closure h' y c"
   by (induction c) simp_all
@@ -68,9 +72,9 @@ lemma [simp]: "halloc h c = (h', v) \<Longrightarrow> stack_contains h env \<Lon
     map (unheap_closure h') env = map (unheap_closure h) env"
   by (induction env) (simp_all del: unheap_closure.simps)
 
-lemma [simp]: "halloc h c = (h', v) \<Longrightarrow> env_contains h env \<Longrightarrow> heap_all (bounded_closure h) h \<Longrightarrow>
-    map (map (unheap_closure h')) env = map (map (unheap_closure h)) env"
-  by (induction env) (simp_all del: unheap_closure.simps)
+lemma [simp]: "halloc h c = (h', v) \<Longrightarrow> env_contains h (map fst sfs) \<Longrightarrow> 
+    heap_all (bounded_closure h) h \<Longrightarrow> unheap_stack h' sfs = unheap_stack h sfs"
+  by (induction sfs rule: unheap_stack.induct) (simp_all del: unheap_closure.simps)
 
 lemma [simp]: "halloc h (HLam env p) = (h', v) \<Longrightarrow> stack_contains h env \<Longrightarrow> 
     heap_all (bounded_closure h) h \<Longrightarrow> unheap_closure h' v = BLam (map (unheap_closure h) env) p"
@@ -82,12 +86,12 @@ lemma [simp]: "hlookup h v = HLam env pc \<Longrightarrow> heap_all (bounded_clo
 
 lemma [simp]: "\<Sigma>\<^sub>h \<leadsto>\<^sub>h \<Sigma>\<^sub>h' \<Longrightarrow> heap_structured \<Sigma>\<^sub>h \<Longrightarrow> heap_structured \<Sigma>\<^sub>h'"
 proof (induction \<Sigma>\<^sub>h \<Sigma>\<^sub>h' rule: evalh.induct)
-  case (evh_apply cd pc h v2 env pc' v1 vs envs pcs)
+  case (evh_apply cd pc h v2 env pc' v1 vs sfs)
   hence "hlookup h v2 = HLam env pc' \<and> heap_all (bounded_closure h) h \<and> hcontains h v2" by simp
   hence "bounded_closure h v2 (HLam env pc')" by (metis heap_lookup_all)
   with evh_apply show ?case by simp
 next
-  case (evh_jump cd pc h v2 env' pc' v1 vs env envs pcs)
+  case (evh_jump cd pc h v2 env' pc' v1 vs env sfs)
   hence "hlookup h v2 = HLam env' pc' \<and> heap_all (bounded_closure h) h \<and> hcontains h v2" by simp
   hence "bounded_closure h v2 (HLam env' pc')" by (metis heap_lookup_all)
   with evh_jump show ?case by simp
@@ -99,10 +103,13 @@ lemma [simp]: "iter (\<leadsto>\<^sub>h) \<Sigma>\<^sub>h \<Sigma>\<^sub>h' \<Lo
 theorem correcth [simp]: "\<Sigma>\<^sub>h \<leadsto>\<^sub>h \<Sigma>\<^sub>h' \<Longrightarrow> heap_structured \<Sigma>\<^sub>h \<Longrightarrow> unheap \<Sigma>\<^sub>h \<leadsto>\<^sub>b unheap \<Sigma>\<^sub>h'"
   by (induction \<Sigma>\<^sub>h \<Sigma>\<^sub>h' rule: evalh.induct) simp_all
 
-lemma unheap_backwards [simp]: "BS vs envs pcs cd = unheap \<Sigma>\<^sub>h \<Longrightarrow> \<exists>h vs' envs'. 
-  \<Sigma>\<^sub>h = HS h vs' envs' pcs cd \<and> vs = map (unheap_closure h) vs' \<and> 
-    envs = map (map (unheap_closure h)) envs'"
-  by (induction \<Sigma>\<^sub>h) simp_all
+lemma unheap_backwards [simp]: "BS vs ((env, pc) # sfs) cd = unheap \<Sigma>\<^sub>h \<Longrightarrow> \<exists>h vs' env' sfs'. 
+  \<Sigma>\<^sub>h = HS h vs' ((env', pc) # sfs') cd \<and> vs = map (unheap_closure h) vs' \<and> 
+    env = map (unheap_closure h) env' \<and> sfs = unheap_stack h sfs'"
+proof (induction \<Sigma>\<^sub>h)
+  case (HS h vs' sfs' cd')
+  thus ?case by (induction h sfs' rule: unheap_stack.induct) (simp_all del: unheap_closure.simps)
+qed 
 
 lemma [simp]: "unheap_closure h v = BLam env pc \<Longrightarrow> hcontains h v \<Longrightarrow> 
   heap_all (bounded_closure h) h \<Longrightarrow> 
@@ -112,68 +119,63 @@ lemma [simp]: "unheap_closure h v = BLam env pc \<Longrightarrow> hcontains h v 
 theorem completeh [simp]: "unheap \<Sigma>\<^sub>h \<leadsto>\<^sub>b \<Sigma>\<^sub>b' \<Longrightarrow> heap_structured \<Sigma>\<^sub>h \<Longrightarrow> 
   \<exists>\<Sigma>\<^sub>h'. \<Sigma>\<^sub>h \<leadsto>\<^sub>h \<Sigma>\<^sub>h' \<and> \<Sigma>\<^sub>b' = unheap \<Sigma>\<^sub>h'"
 proof (induction "unheap \<Sigma>\<^sub>h" \<Sigma>\<^sub>b' rule: evalb.induct)
-  case (evb_lookup cd pc x env v vs envs pcs)
-  then obtain h vs' envs'' where "\<Sigma>\<^sub>h = HS h vs' envs'' (Suc pc # pcs) cd \<and> 
-    vs = map (unheap_closure h) vs' \<and> env # envs = map (map (unheap_closure h)) envs''" by fastforce
-  moreover then obtain env' envs' where "envs'' = env' # envs' \<and> 
-    env = map (unheap_closure h) env' \<and> envs = map (map (unheap_closure h)) envs'" by fastforce
-  moreover with evb_lookup obtain v' where "lookup env' x = Some v' \<and> v = unheap_closure h v'" 
-    by fastforce
-  moreover with evb_lookup have "HS h vs' (env' # envs') (Suc pc # pcs) cd \<leadsto>\<^sub>h 
-    HS h (v' # vs') (env' # envs') (pc # pcs) cd" by simp
-  ultimately show ?case by fastforce
-next
-  case (evb_pushcon cd pc k vs envs pcs)
-  moreover then obtain h vs' envs' where "\<Sigma>\<^sub>h = HS h vs' envs' (Suc pc # pcs) cd \<and> 
-    vs = map (unheap_closure h) vs' \<and> envs = map (map (unheap_closure h)) envs'" by fastforce
-  moreover obtain h' v where "halloc h (HConst k) = (h', v)" by fastforce
-  moreover with evb_pushcon have "HS h vs' envs' (Suc pc # pcs) cd \<leadsto>\<^sub>h 
-    HS h' (v # vs') envs' (pc # pcs) cd" by simp
-  ultimately show ?case by fastforce
-next
-  case (evb_pushlam cd pc pc' vs env envs pcs)
-  moreover then obtain h vs' envs'' where "\<Sigma>\<^sub>h = HS h vs' envs'' (Suc pc # pcs) cd \<and> 
-    vs = map (unheap_closure h) vs' \<and> env # envs = map (map (unheap_closure h)) envs''" by fastforce
-  moreover then obtain env' envs' where "envs'' = env' # envs' \<and> 
-    env = map (unheap_closure h) env' \<and> envs = map (map (unheap_closure h)) envs'" by fastforce
-  moreover obtain h' v where "halloc h (HLam env' pc') = (h', v)" by fastforce
-  moreover with evb_pushlam have "HS h vs' (env' # envs') (Suc pc # pcs) cd \<leadsto>\<^sub>h 
-    HS h' (v # vs') (env' # envs') (pc # pcs) cd" by simp
-  ultimately show ?case by fastforce
-next
-  case (evb_apply cd pc v env pc' vs envs pcs)
-  then obtain h vs'' envs' where S: "\<Sigma>\<^sub>h = HS h vs'' envs' (Suc pc # pcs) cd \<and> 
-    v # BLam env pc' # vs = map (unheap_closure h) vs'' \<and> envs = map (map (unheap_closure h)) envs'" 
+  case (evb_lookup cd pc x env v vs sfs)
+  then obtain h vs' env' sfs' where "\<Sigma>\<^sub>h = HS h vs' ((env', Suc pc) # sfs') cd \<and> 
+    vs = map (unheap_closure h) vs' \<and> env = map (unheap_closure h) env' \<and> sfs = unheap_stack h sfs'" 
       by fastforce
+  moreover with evb_lookup obtain vv where "lookup env' x = Some vv \<and> v = unheap_closure h vv" 
+    by fastforce
+  moreover with evb_lookup have "HS h vs' ((env', Suc pc) # sfs') cd \<leadsto>\<^sub>h 
+    HS h (vv # vs') ((env', pc) # sfs') cd" by simp
+  ultimately show ?case by fastforce
+next
+  case (evb_pushcon cd pc k vs env sfs)
+  moreover then obtain h vs' env' sfs' where "\<Sigma>\<^sub>h = HS h vs' ((env', Suc pc) # sfs') cd \<and> 
+    vs = map (unheap_closure h) vs' \<and> env = map (unheap_closure h) env' \<and> sfs = unheap_stack h sfs'" 
+      by fastforce
+  moreover obtain h' v where "halloc h (HConst k) = (h', v)" by fastforce
+  moreover with evb_pushcon have "HS h vs' ((env', Suc pc) # sfs') cd \<leadsto>\<^sub>h 
+    HS h' (v # vs') ((env', pc) # sfs') cd" by simp
+  ultimately show ?case by fastforce
+next
+  case (evb_pushlam cd pc pc' vs env sfs)
+  moreover then obtain h vs' env' sfs' where "\<Sigma>\<^sub>h = HS h vs' ((env', Suc pc) # sfs') cd \<and> 
+    vs = map (unheap_closure h) vs' \<and> env = map (unheap_closure h) env' \<and> sfs = unheap_stack h sfs'" 
+      by fastforce
+  moreover obtain h' v where "halloc h (HLam env' pc') = (h', v)" by fastforce
+  moreover with evb_pushlam have "HS h vs' ((env', Suc pc) # sfs') cd \<leadsto>\<^sub>h 
+    HS h' (v # vs') ((env', pc) # sfs') cd" by simp
+  ultimately show ?case by fastforce
+next
+  case (evb_apply cd pc v env' pc' vs env sfs)
+  then obtain h vs'' envh sfs' where S: "\<Sigma>\<^sub>h = HS h vs'' ((envh, Suc pc) # sfs') cd \<and> 
+    v # BLam env' pc' # vs = map (unheap_closure h) vs'' \<and> env = map (unheap_closure h) envh \<and> 
+      sfs = unheap_stack h sfs'" by fastforce
   moreover then obtain v1 v2 vs' where "vs'' = v1 # v2 # vs' \<and> v = unheap_closure h v1 \<and> 
-    BLam env pc' = unheap_closure h v2 \<and> vs = map (unheap_closure h) vs'" by fastforce
-  moreover with evb_apply S obtain env' where "hlookup h v2 = HLam env' pc' \<and> 
-    env = map (unheap_closure h) env'" by fastforce
-  moreover with evb_apply have "HS h (v1 # v2 # vs') envs' (Suc pc # pcs) cd \<leadsto>\<^sub>h 
-    HS h vs' ((v1 # env') # envs') (pc' # pc # pcs) cd" by simp
+    BLam env' pc' = unheap_closure h v2 \<and> vs = map (unheap_closure h) vs'" by fastforce
+  moreover with evb_apply S obtain envh' where H: "hlookup h v2 = HLam envh' pc' \<and> 
+    env' = map (unheap_closure h) envh'" by fastforce
+  moreover with evb_apply have "HS h (v1 # v2 # vs') ((envh, Suc pc) # sfs') cd \<leadsto>\<^sub>h 
+    HS h vs' ((v1 # envh', pc') # (envh, pc) # sfs') cd" by simp
   ultimately show ?case by fastforce
 next
-  case (evb_return cd pc vs env envs pcs)
-  then obtain h vs' envs'' where "\<Sigma>\<^sub>h = HS h vs' envs'' (Suc pc # pcs) cd \<and> 
-    vs = map (unheap_closure h) vs' \<and> env # envs = map (map (unheap_closure h)) envs''" by fastforce
-  moreover then obtain env' envs' where "envs'' = env' # envs' \<and> 
-    env = map (unheap_closure h) env' \<and> envs = map (map (unheap_closure h)) envs'" by fastforce
-  moreover from evb_return have "HS h vs' (env' # envs') (Suc pc # pcs) cd \<leadsto>\<^sub>h 
-    HS h vs' envs' pcs cd" by simp
+  case (evb_return cd pc vs env sfs)
+  then obtain h vs' env' sfs' where "\<Sigma>\<^sub>h = HS h vs' ((env', Suc pc) # sfs') cd \<and> 
+    vs = map (unheap_closure h) vs' \<and> env = map (unheap_closure h) env' \<and> sfs = unheap_stack h sfs'" 
+      by fastforce
+  moreover from evb_return have "HS h vs' ((env', Suc pc) # sfs') cd \<leadsto>\<^sub>h HS h vs' sfs' cd" by simp
   ultimately show ?case by fastforce
 next
-  case (evb_jump cd pc v env' pc' vs env envs pcs)
-  then obtain h vs'' envs'' where S: "\<Sigma>\<^sub>h = HS h vs'' envs'' (Suc pc # pcs) cd \<and> 
-    v # BLam env' pc' # vs = map (unheap_closure h) vs'' \<and> 
-      env # envs = map (map (unheap_closure h)) envs''" by fastforce
-  moreover then obtain envh envs' where "envs'' = envh # envs' \<and> 
-    env = map (unheap_closure h) envh \<and> envs = map (map (unheap_closure h)) envs'" by fastforce
+  case (evb_jump cd pc v env' pc' vs env sfs)
+  then obtain h vs'' envh sfs' where S: "\<Sigma>\<^sub>h = HS h vs'' ((envh, Suc pc) # sfs') cd \<and> 
+    v # BLam env' pc' # vs = map (unheap_closure h) vs'' \<and> env = map (unheap_closure h) envh \<and> 
+      sfs = unheap_stack h sfs'" by fastforce
   moreover from S obtain v1 v2 vs' where "vs'' = v1 # v2 # vs' \<and> v = unheap_closure h v1 \<and> 
     BLam env' pc' = unheap_closure h v2 \<and> vs = map (unheap_closure h) vs'" by fastforce
   moreover with evb_jump S obtain envh' where "hlookup h v2 = HLam envh' pc' \<and> 
     env' = map (unheap_closure h) envh'" by fastforce
-  moreover with evb_jump have "HS h (v1 # v2 # vs') (envh # envs') (Suc pc # pcs) cd \<leadsto>\<^sub>h 
-    HS h vs' ((v1 # envh') # envs') (pc' # pcs) cd" by simp
+  moreover with evb_jump have "HS h (v1 # v2 # vs') ((envh, Suc pc) # sfs') cd \<leadsto>\<^sub>h 
+    HS h vs' ((v1 # envh', pc') # sfs') cd" by simp
   ultimately show ?case by fastforce
 qed
 
