06TailCall/TailCall.thy
@@ -1,0 +1,67 @@
+theory TailCall
+  imports "../00Utils/Environment"
+begin
+
+datatype tco_return =
+    TCOReturn
+  | TCOJump
+
+datatype tco_code = 
+  TCOLookup nat
+  | TCOPushCon nat
+  | TCOPushLam "tco_code list" tco_return
+  | TCOApply
+
+datatype tco_closure = 
+  TCOConst nat
+  | TCOLam "tco_closure list" "tco_code list" tco_return
+
+type_synonym tco_stack_frame = "tco_closure list \<times> tco_code list \<times> tco_return"
+
+datatype tco_code_state = TCOS "tco_closure list" "tco_stack_frame list"
+
+inductive evaltco :: "tco_code_state \<Rightarrow> tco_code_state \<Rightarrow> bool" (infix "\<leadsto>\<^sub>t\<^sub>c\<^sub>o" 50) where
+  evtco_lookup [simp]: "lookup env x = Some v \<Longrightarrow> 
+    TCOS vs ((env, TCOLookup x # cd, r) # sfs) \<leadsto>\<^sub>t\<^sub>c\<^sub>o TCOS (v # vs) ((env, cd, r) # sfs)"
+| evtco_pushcon [simp]: "TCOS vs ((env, TCOPushCon k # cd, r) # sfs) \<leadsto>\<^sub>t\<^sub>c\<^sub>o 
+    TCOS (TCOConst k # vs) ((env, cd, r) # sfs)"
+| evtco_pushlam [simp]: "TCOS vs ((env, TCOPushLam cd' r' # cd, r) # sfs) \<leadsto>\<^sub>t\<^sub>c\<^sub>o 
+    TCOS (TCOLam env cd' r' # vs) ((env, cd, r) # sfs)"
+| evtco_apply [simp]: "TCOS (v # TCOLam env cd' r' # vs) ((env, TCOApply # cd, r) # sfs) \<leadsto>\<^sub>t\<^sub>c\<^sub>o 
+    TCOS vs ((v # env, cd', r') # (env, cd, r) # sfs)"
+| evtco_return [simp]: "TCOS vs ((env, [], TCOReturn) # sfs) \<leadsto>\<^sub>t\<^sub>c\<^sub>o TCOS vs sfs"
+| evtco_jump [simp]: "TCOS (v # TCOLam env' cd' r' # vs) ((env, [], TCOJump) # sfs) \<leadsto>\<^sub>t\<^sub>c\<^sub>o 
+    TCOS vs ((v # env', cd', r') # sfs)"
+
+theorem determinismt: "\<Sigma> \<leadsto>\<^sub>t\<^sub>c\<^sub>o \<Sigma>' \<Longrightarrow> \<Sigma> \<leadsto>\<^sub>t\<^sub>c\<^sub>o \<Sigma>'' \<Longrightarrow> \<Sigma>' = \<Sigma>''"
+proof (induction \<Sigma> \<Sigma>' rule: evaltco.induct)
+  case (evtco_lookup env x v vs cd r sfs)
+  from evtco_lookup(2, 1) show ?case 
+    by (induction "TCOS vs ((env, TCOLookup x # cd, r) # sfs)" \<Sigma>'' rule: evaltco.induct) simp_all 
+next
+  case (evtco_pushcon vs env k cd r sfs)
+  thus ?case 
+    by (induction "TCOS vs ((env, TCOPushCon k # cd, r) # sfs)" \<Sigma>'' rule: evaltco.induct) simp_all 
+next
+  case (evtco_pushlam vs env cd' r' cd r sfs)
+  thus ?case 
+    by (induction "TCOS vs ((env, TCOPushLam cd' r' # cd, r) # sfs)" \<Sigma>'' rule: evaltco.induct) 
+       simp_all 
+next
+  case (evtco_apply v env cd' r' vs cd r sfs)
+  thus ?case 
+    by (induction "TCOS (v # TCOLam env cd' r' # vs) ((env, TCOApply # cd, r) # sfs)" \<Sigma>'' 
+        rule: evaltco.induct) 
+       simp_all 
+next
+  case (evtco_return vs env sfs)
+  thus ?case by (induction "TCOS vs ((env, [], TCOReturn) # sfs)" \<Sigma>'' rule: evaltco.induct) simp_all 
+next
+  case (evtco_jump v env' cd' r' vs env sfs)
+  thus ?case 
+    by (induction "TCOS (v # TCOLam env' cd' r' # vs) ((env, [], TCOJump) # sfs)" \<Sigma>''
+        rule: evaltco.induct) 
+       simp_all 
+qed
+
+end
