07FlatCode/ByteCode.thy
@@ -1,0 +1,70 @@
+theory ByteCode
+  imports "../00Utils/Environment" "../00Utils/Iteration"
+begin
+
+datatype byte_code = 
+  BLookup nat
+  | BPushCon nat
+  | BPushLam nat
+  | BApply
+  | BReturn
+  | BJump
+
+datatype bclosure = 
+  BConst nat
+  | BLam "bclosure list" nat
+
+datatype byte_code_state = 
+  BS "bclosure list" "(bclosure list \<times> nat) list" (code: "byte_code list")
+
+inductive evalb :: "byte_code_state \<Rightarrow> byte_code_state \<Rightarrow> bool" (infix "\<leadsto>\<^sub>b" 50) where
+  evb_lookup [simp]: "cd ! pc = BLookup x \<Longrightarrow> lookup env x = Some v \<Longrightarrow> 
+    BS vs ((env, Suc pc) # sfs) cd \<leadsto>\<^sub>b BS (v # vs) ((env, pc) # sfs) cd"
+| evb_pushcon [simp]: "cd ! pc = BPushCon k \<Longrightarrow> 
+    BS vs ((env, Suc pc) # sfs) cd \<leadsto>\<^sub>b BS (BConst k # vs) ((env, pc) # sfs) cd"
+| evb_pushlam [simp]: "cd ! pc = BPushLam pc' \<Longrightarrow> 
+    BS vs ((env, Suc pc) # sfs) cd \<leadsto>\<^sub>b BS (BLam env pc' # vs) ((env, pc) # sfs) cd"
+| evb_apply [simp]: "cd ! pc = BApply \<Longrightarrow> 
+    BS (v # BLam env' pc' # vs) ((env, Suc pc) # sfs) cd \<leadsto>\<^sub>b 
+      BS vs ((v # env', pc') # (env, pc) # sfs) cd"
+| evb_return [simp]: "cd ! pc = BReturn \<Longrightarrow> BS vs ((env, Suc pc) # sfs) cd \<leadsto>\<^sub>b BS vs sfs cd"
+| evb_jump [simp]: "cd ! pc = BJump \<Longrightarrow> 
+    BS (v # BLam env' pc' # vs) ((env, Suc pc) # sfs) cd \<leadsto>\<^sub>b 
+      BS vs ((v # env', pc') # sfs) cd"
+
+theorem determinismb: "\<Sigma> \<leadsto>\<^sub>b \<Sigma>' \<Longrightarrow> \<Sigma> \<leadsto>\<^sub>b \<Sigma>'' \<Longrightarrow> \<Sigma>' = \<Sigma>''"
+proof (induction \<Sigma> \<Sigma>' rule: evalb.induct)
+  case (evb_lookup cd pc x env v vs sfs)
+  from evb_lookup(3, 1, 2) show ?case 
+    by (induction "BS vs ((env, Suc pc) # sfs) cd" \<Sigma>'' rule: evalb.induct) simp_all 
+next
+  case (evb_pushcon cd pc k vs env sfs)
+  from evb_pushcon(2, 1) show ?case 
+    by (induction "BS vs ((env, Suc pc) # sfs) cd" \<Sigma>'' rule: evalb.induct) simp_all 
+next
+  case (evb_pushlam cd pc pc' vs env sfs)
+  from evb_pushlam(2, 1) show ?case 
+    by (induction "BS vs ((env, Suc pc) # sfs) cd" \<Sigma>'' rule: evalb.induct) simp_all 
+next
+  case (evb_apply cd pc v env' pc' vs env sfs)
+  from evb_apply(2, 1) show ?case 
+    by (induction "BS (v # BLam env' pc' # vs) ((env, Suc pc) # sfs) cd" \<Sigma>'' rule: evalb.induct) 
+       simp_all 
+next
+  case (evb_return cd pc vs env sfs)
+  from evb_return(2, 1) show ?case 
+    by (induction "BS vs ((env, Suc pc) # sfs) cd" \<Sigma>'' rule: evalb.induct) simp_all 
+next
+  case (evb_jump cd pc v env' pc' vs env sfs)
+  from evb_jump(2, 1) show ?case 
+    by (induction "BS (v # BLam env' pc' # vs) ((env, Suc pc) # sfs) cd" \<Sigma>'' rule: evalb.induct) 
+       simp_all 
+qed
+
+lemma [simp]: "\<Sigma> \<leadsto>\<^sub>b \<Sigma>' \<Longrightarrow> code \<Sigma> = code \<Sigma>'"
+  by (induction \<Sigma> \<Sigma>' rule: evalb.induct) simp_all
+
+lemma [simp]: "iter (\<leadsto>\<^sub>b) \<Sigma> \<Sigma>' \<Longrightarrow> code \<Sigma> = code \<Sigma>'"
+  by (induction \<Sigma> \<Sigma>' rule: iter.induct) simp_all
+
+end
