08HeapMemory/HeapMemory.thy
@@ -1,0 +1,63 @@
+theory HeapMemory
+  imports "../07FlatCode/ByteCode" Heap
+begin
+
+datatype hclosure = 
+  HConst nat
+  | HLam "ptr list" nat
+
+datatype heap_state = 
+  HS "hclosure heap" "ptr list" "(ptr list \<times> nat) list" (code: "byte_code list")
+
+inductive evalh :: "heap_state \<Rightarrow> heap_state \<Rightarrow> bool" (infix "\<leadsto>\<^sub>h" 50) where
+  evh_lookup [simp]: "cd ! pc = BLookup x \<Longrightarrow> lookup env x = Some v \<Longrightarrow> 
+    HS h vs ((env, Suc pc) # sfs) cd \<leadsto>\<^sub>h HS h (v # vs) ((env, pc) # sfs) cd"
+| evh_pushcon [simp]: "cd ! pc = BPushCon k \<Longrightarrow> halloc h (HConst k) = (h', v) \<Longrightarrow>
+    HS h vs ((env, Suc pc) # sfs) cd \<leadsto>\<^sub>h HS h' (v # vs) ((env, pc) # sfs) cd"
+| evh_pushlam [simp]: "cd ! pc = BPushLam pc' \<Longrightarrow> halloc h (HLam env pc') = (h', v) \<Longrightarrow>
+    HS h vs ((env, Suc pc) # sfs) cd \<leadsto>\<^sub>h HS h' (v # vs) ((env, pc) # sfs) cd"
+| evh_apply [simp]: "cd ! pc = BApply \<Longrightarrow> hlookup h v2 = HLam env' pc' \<Longrightarrow>
+    HS h (v1 # v2 # vs) ((env, Suc pc) # sfs) cd \<leadsto>\<^sub>h
+      HS h vs ((v1 # env', pc') # (env, pc) # sfs) cd"
+| evh_return [simp]: "cd ! pc = BReturn \<Longrightarrow> 
+    HS h vs ((env, Suc pc) # sfs) cd \<leadsto>\<^sub>h HS h vs sfs cd"
+| evh_jump [simp]: "cd ! pc = BJump \<Longrightarrow> hlookup h v2 = HLam env' pc' \<Longrightarrow>
+    HS h (v1 # v2 # vs) ((env, Suc pc) # sfs) cd \<leadsto>\<^sub>h 
+      HS h vs ((v1 # env', pc') # sfs) cd"
+
+theorem determinismh: "\<Sigma> \<leadsto>\<^sub>h \<Sigma>' \<Longrightarrow> \<Sigma> \<leadsto>\<^sub>h \<Sigma>'' \<Longrightarrow> \<Sigma>' = \<Sigma>''"
+proof (induction \<Sigma> \<Sigma>' rule: evalh.induct)
+  case (evh_lookup cd pc x env v h vs sfs)
+  from evh_lookup(3, 1, 2) show ?case 
+    by (induction "HS h vs ((env, Suc pc) # sfs) cd" \<Sigma>'' rule: evalh.induct) simp_all 
+next
+  case (evh_pushcon cd pc k h h' v vs env sfs)
+  from evh_pushcon(3, 1, 2) show ?case 
+    by (induction "HS h vs ((env, Suc pc) # sfs) cd" \<Sigma>'' rule: evalh.induct) simp_all 
+next
+  case (evh_pushlam cd pc pc' h env h' v vs sfs)
+  from evh_pushlam(3, 1, 2) show ?case 
+    by (induction "HS h vs ((env, Suc pc) # sfs) cd" \<Sigma>'' rule: evalh.induct) simp_all 
+next
+  case (evh_apply cd pc h v2 env' pc' v1 vs env sfs)
+  from evh_apply(3, 1, 2) show ?case 
+    by (induction "HS h (v1 # v2 # vs) ((env, Suc pc) # sfs) cd" \<Sigma>'' rule: evalh.induct) 
+       simp_all 
+next
+  case (evh_return cd pc h vs env sfs)
+  from evh_return(2, 1) show ?case 
+    by (induction "HS h vs ((env, Suc pc) # sfs) cd" \<Sigma>'' rule: evalh.induct) simp_all 
+next
+  case (evh_jump cd pc h v2 env' pc' v1 vs env sfs)
+  from evh_jump(3, 1, 2) show ?case 
+    by (induction "HS h (v1 # v2 # vs) ((env, Suc pc) # sfs) cd" \<Sigma>'' rule: evalh.induct) 
+       simp_all 
+qed
+
+lemma [simp]: "\<Sigma> \<leadsto>\<^sub>h \<Sigma>' \<Longrightarrow> code \<Sigma> = code \<Sigma>'"
+  by (induction \<Sigma> \<Sigma>' rule: evalh.induct) simp_all
+
+lemma [simp]: "iter (\<leadsto>\<^sub>h) \<Sigma> \<Sigma>' \<Longrightarrow> code \<Sigma> = code \<Sigma>'"
+  by (induction \<Sigma> \<Sigma>' rule: iter.induct) simp_all
+
+end
